sciostar/Compiler.ModelStlc.fst
@@ -84,8 +84,8 @@ type whole_src = mst:mstate & post:(trace -> int -> trace -> Type0) & (unit -> M
 let link_src (#i:src_interface) (p:prog_src i) (c:ctx_src i) : whole_src = 
   (| i.mst, i.psi,  p #AllOps (c #AllOps (inst_io_lib i.pi) (make_dcs_eff i.ct_dcs)) |)
 
-val beh_src : whole_src ^-> trace_property #event
-let beh_src = on_domain whole_src (fun (| mst, _, ws |) -> beh mst ws)
+val beh_src : whole_src -> trace_property #event
+let beh_src = fun (| mst, _, ws |) -> beh mst ws
 
 let src_language : language (trace_property #event) = {
   interface = src_interface;
@@ -104,8 +104,8 @@ let link_tgt (#i:tgt_interface) (p:prog_tgt i) (c:ctx_tgt i) : whole_tgt =
   let c' = bt_ctx e i.ct h #AllOps #i.sgm #i.mst sec_io in
   (| i.mst , p c' |)
 
-val beh_tgt : whole_tgt ^-> trace_property #event
-let beh_tgt = on_domain whole_tgt (fun (| mst, wt |) -> beh mst wt)
+val beh_tgt : whole_tgt -> trace_property #event
+let beh_tgt = fun (| mst, wt |) -> beh mst wt
 
 let tgt_language : language (trace_property #event) = {
   interface = tgt_interface;
